[minor] [verif] Factored out range generation from SFI.

sfi/abstract.v
@@ -1,6 +1,7 @@
 Require Import List Arith Sorted Bool.
 Require Import Coq.Classes.SetoidDec.
-Require Import lib.utils concrete.common lib.ordered list_utils set_utils.
+Require Import lib.utils concrete.common lib.ordered.
+Require Import list_utils set_utils ranges.
 
 Import DoNotation.
 
@@ -29,134 +30,6 @@ Local Notation value := word.
 (* I want to use S as a variable. *)
 Let S := Datatypes.S.
 Local Notation Suc := Datatypes.S.
-
-(**** RANGE ****)
-(* TODO abstract and reify *)
-Require Import ZArith.
-
-Fixpoint range' (meas : nat) (l h : word) : list word :=
-  match meas , l <=> h with
-    | O         , _  => []
-    | Suc meas' , Lt => l :: range' meas' (l + 1) h
-    | Suc meas' , Eq => [l]
-    | Suc meas' , Gt => []
-  end.
-
-Lemma addw_succ : forall w1 w2,
-  w1 < w2 -> word_to_Z (w1 + Z_to_word 1)%w = (word_to_Z w1 + 1)%Z.
-Proof.
-  intros x y LT.
-  rewrite <- (word_to_ZK x) at 1; rewrite <- (word_to_ZK 1).
-  rewrite addwP.
-  repeat rewrite Z_to_wordK;
-    try solve [ reflexivity
-              | generalize min_word_bound, max_word_bound; omega ].
-  assert (word_to_Z min_word <= word_to_Z x)%Z by
-    (rewrite <- word_to_Z_le; apply lew_min).
-  assert (word_to_Z y <= word_to_Z max_word)%Z by 
-    (rewrite <- word_to_Z_le; apply lew_max).
-  assert (word_to_Z x < word_to_Z max_word)%Z by
-    (apply word_to_Z_lt in LT; omega).
-  omega.
-Qed.  
-
-Lemma lebw_succ : forall x y, x < y -> x <? x + 1 = true.
-Proof.
-  intros x y LT. apply addw_succ in LT.
-  rewrite word_to_Z_ltb, LT, Z.ltb_lt; omega.
-Qed.
-
-Theorem range'_set : forall meas l h,
-  is_set (range' meas l h) = true.
-Proof.
-  induction meas as [|meas]; simpl; [reflexivity|].
-  intros l h; destruct (l <=> h) eqn:CMP; try reflexivity.
-  simpl; rewrite IHmeas.
-  destruct meas; simpl; [reflexivity|].
-  destruct (l + 1 <=> h) eqn:CMP';
-    solve [ reflexivity | rewrite andb_true_r; eapply lebw_succ; eassumption ].
-Qed.
-
-Theorem range'_elts_ok : forall meas l h e,
-  In e (range' meas l h) -> l <= e <= h.
-Proof.
-  induction meas as [|meas]; [inversion 1|].
-  simpl; intros until 0; intros IN.
-  destruct (l <=> h) eqn:CMP; simpl in *.
-  - apply compare_eq in CMP; destruct IN as [EQ|[]];
-      repeat progress subst; auto 2 with ordered.
-  - destruct IN as [EQ | IN]; subst; auto with ordered.
-    apply IHmeas in IN; destruct IN as [LT LE].
-    assert (l < l + 1) by (eapply ltb_lt,lebw_succ; eassumption).
-    split; eauto with ordered.
-  - inversion IN.
-Qed.
-
-Definition range (l h : word) :=
-  range' (Z.to_nat ((word_to_Z h - word_to_Z l) + 1)%Z) l h.
-
-Corollary range_set : forall l h, is_set (range l h) = true.
-Proof. intros until 0; apply range'_set. Qed.
-Hint Resolve range_set.
-
-Corollary range_elts_ok : forall l h e,
-  In e (range l h) -> l <= e <= h.
-Proof. intros until 0; apply range'_elts_ok. Qed.
-
-Lemma addw_le : forall x y,
-  x < y -> x + 1 <= y.
-Proof.
-  intros x y LT.
-  apply word_to_Z_le.
-  erewrite addw_succ by eassumption.
-  apply word_to_Z_lt in LT.
-  omega.
-Qed.
-
-Theorem range_elts_all : forall l h e,
-  l <= e <= h -> In e (range l h).
-Proof.
-  unfold range; intros l h e [LE EH];
-    assert (LH : l <= h) by eauto with ordered.
-  remember (Z.to_nat ((word_to_Z h - word_to_Z l) + 1)%Z) as meas eqn:meas_def'.
-  assert (meas_def : meas = S (Z.to_nat (word_to_Z h - word_to_Z l))). {
-    rewrite Z2Nat.inj_add in meas_def'; try solve [vm_compute; inversion 1].
-    - rewrite plus_comm in meas_def'; simpl in meas_def'; exact meas_def'.
-    - apply Z.le_0_sub, word_to_Z_le; exact LH.
-  }
-  clear meas_def'; gdep e; gdep h; gdep l; induction meas; intros;
-    simpl in *; inversion meas_def; subst; clear meas_def.
-  destruct (l <=> h) eqn:CMP.
-  - apply compare_eq in CMP; apply le__lt_or_eq in EH; apply le__lt_or_eq in LE;
-      subst; destruct EH,LE; auto with ordered.
-    elim (lt_asym h e); assumption.
-  - simpl. apply le__lt_or_eq in LE; destruct LE as [LE | LE]; auto.
-    right; apply IHmeas; eauto using addw_le.
-    erewrite addw_succ by eassumption.
-    replace (word_to_Z h - (word_to_Z l + 1))%Z
-       with (word_to_Z h - word_to_Z l - 1)%Z
-         by omega.
-    rewrite <- Z2Nat.inj_succ.
-    + f_equal; omega.
-    + rewrite Z.sub_1_r; apply Zlt_0_le_0_pred, Z.lt_0_sub, word_to_Z_lt;
-        exact CMP.
-  - contradiction.
-Qed.
-
-Corollary range_elts : forall l h e,
-  In e (range l h) <-> l <= e <= h.
-Proof. split; [apply range_elts_ok | apply range_elts_all]. Qed.
-
-Corollary range_empty : forall l h,
-  range l h = [] <-> l > h.
-Proof.
-  intros; rewrite nil_iff_not_in; split.
-  - intros NOT_IN; apply gt_not_le; intros LE.
-    apply NOT_IN with l, range_elts; auto with ordered.
-  - intros GT e IN. apply range_elts in IN.
-    destruct IN; assert (l <= h) by eauto 2 with ordered; auto.
-Qed.
-(***** END RANGE *****)
 
 Implicit Type pc : value.
 
@@ -909,7 +782,7 @@ Hint Resolve isolate_create_set_is_set.
 
 Theorem isolate_good : forall MM, good_syscall isolate MM = true.
 Proof.
-  clear; unfold isolate, good_syscall; intros MM; simpl.
+  clear - t ops spec; unfold isolate, good_syscall; intros MM; simpl.
   destruct (good_state MM) eqn:GOOD, MM as [pc R M C];
     [unfold good_state in *; simpl in * | reflexivity].
   rewrite andb_true_iff in GOOD; destruct GOOD as [EICO GOOD].
