sfi/ranges.v
@@ -1,0 +1,142 @@
+Require Import List Bool ZArith.
+Require Import lib.utils concrete.common lib.ordered list_utils set_utils.
+
+Section WithClasses.
+
+Context {t    : machine_types}
+        {ops  : machine_ops t}
+        {spec : machine_ops_spec ops}.
+
+Import ListNotations.
+Local Notation word := (word t).
+Open Scope word_scope.
+
+(* TODO abstract and reify *)
+Require Import ZArith.
+
+Fixpoint range' (meas : nat) (l h : word) : list word :=
+  match meas , l <=> h with
+    | O       , _  => []
+    | S meas' , Lt => l :: range' meas' (l + 1) h
+    | S meas' , Eq => [l]
+    | S meas' , Gt => []
+  end.
+
+Lemma addw_succ : forall w1 w2,
+  w1 < w2 -> word_to_Z (w1 + Z_to_word 1)%w = (word_to_Z w1 + 1)%Z.
+Proof.
+  intros x y LT.
+  rewrite <- (word_to_ZK x) at 1; rewrite <- (word_to_ZK 1).
+  rewrite addwP.
+  repeat rewrite Z_to_wordK;
+    try solve [ reflexivity
+              | generalize min_word_bound, max_word_bound; omega ].
+  assert (word_to_Z min_word <= word_to_Z x)%Z by
+    (rewrite <- word_to_Z_le; apply lew_min).
+  assert (word_to_Z y <= word_to_Z max_word)%Z by 
+    (rewrite <- word_to_Z_le; apply lew_max).
+  assert (word_to_Z x < word_to_Z max_word)%Z by
+    (apply word_to_Z_lt in LT; omega).
+  omega.
+Qed.  
+
+Lemma lebw_succ : forall x y, x < y -> x <? x + 1 = true.
+Proof.
+  intros x y LT. apply addw_succ in LT.
+  rewrite word_to_Z_ltb, LT, Z.ltb_lt; omega.
+Qed.
+
+Theorem range'_set : forall meas l h,
+  is_set (range' meas l h) = true.
+Proof.
+  induction meas as [|meas]; simpl; [reflexivity|].
+  intros l h; destruct (l <=> h) eqn:CMP; try reflexivity.
+  simpl; rewrite IHmeas.
+  destruct meas; simpl; [reflexivity|].
+  destruct (l + 1 <=> h) eqn:CMP';
+    solve [ reflexivity | rewrite andb_true_r; eapply lebw_succ; eassumption ].
+Qed.
+
+Theorem range'_elts_ok : forall meas l h e,
+  In e (range' meas l h) -> l <= e <= h.
+Proof.
+  induction meas as [|meas]; [inversion 1|].
+  simpl; intros until 0; intros IN.
+  destruct (l <=> h) eqn:CMP; simpl in *.
+  - apply compare_eq in CMP; destruct IN as [EQ|[]];
+      repeat progress subst; auto 2 with ordered.
+  - destruct IN as [EQ | IN]; subst; auto with ordered.
+    apply IHmeas in IN; destruct IN as [LT LE].
+    assert (l < l + 1) by (eapply ltb_lt,lebw_succ; eassumption).
+    split; eauto with ordered.
+  - inversion IN.
+Qed.
+
+Definition range (l h : word) :=
+  range' (Z.to_nat ((word_to_Z h - word_to_Z l) + 1)%Z) l h.
+
+Corollary range_set : forall l h, is_set (range l h) = true.
+Proof. intros until 0; apply range'_set. Qed.
+Hint Resolve range_set.
+
+Corollary range_elts_ok : forall l h e,
+  In e (range l h) -> l <= e <= h.
+Proof. intros until 0; apply range'_elts_ok. Qed.
+
+Lemma addw_le : forall x y,
+  x < y -> x + 1 <= y.
+Proof.
+  intros x y LT.
+  apply word_to_Z_le.
+  erewrite addw_succ by eassumption.
+  apply word_to_Z_lt in LT.
+  omega.
+Qed.
+
+Theorem range_elts_all : forall l h e,
+  l <= e <= h -> In e (range l h).
+Proof.
+  unfold range; intros l h e [LE EH];
+    assert (LH : l <= h) by eauto with ordered.
+  remember (Z.to_nat ((word_to_Z h - word_to_Z l) + 1)%Z) as meas eqn:meas_def'.
+  assert (meas_def : meas = S (Z.to_nat (word_to_Z h - word_to_Z l))). {
+    rewrite Z2Nat.inj_add in meas_def'; try solve [vm_compute; inversion 1].
+    - rewrite plus_comm in meas_def'; simpl in meas_def'; exact meas_def'.
+    - apply Z.le_0_sub, word_to_Z_le; exact LH.
+  }
+  clear meas_def'; gdep e; gdep h; gdep l; induction meas; intros;
+    simpl in *; inversion meas_def; subst; clear meas_def.
+  destruct (l <=> h) eqn:CMP.
+  - apply compare_eq in CMP; apply le__lt_or_eq in EH; apply le__lt_or_eq in LE;
+      subst; destruct EH,LE; auto with ordered.
+    elim (lt_asym h e); assumption.
+  - simpl. apply le__lt_or_eq in LE; destruct LE as [LE | LE]; auto.
+    right; apply IHmeas; eauto using addw_le.
+    erewrite addw_succ by eassumption.
+    replace (word_to_Z h - (word_to_Z l + 1))%Z
+       with (word_to_Z h - word_to_Z l - 1)%Z
+         by omega.
+    rewrite <- Z2Nat.inj_succ.
+    + f_equal; omega.
+    + rewrite Z.sub_1_r; apply Zlt_0_le_0_pred, Z.lt_0_sub, word_to_Z_lt;
+        exact CMP.
+  - contradiction.
+Qed.
+
+Corollary range_elts : forall l h e,
+  In e (range l h) <-> l <= e <= h.
+Proof. split; [apply range_elts_ok | apply range_elts_all]. Qed.
+
+Corollary range_empty : forall l h,
+  range l h = [] <-> l > h.
+Proof.
+  intros; rewrite nil_iff_not_in; split.
+  - intros NOT_IN; apply gt_not_le; intros LE.
+    apply NOT_IN with l, range_elts; auto with ordered.
+  - intros GT e IN. apply range_elts in IN.
+    destruct IN; assert (l <= h) by eauto 2 with ordered; auto.
+Qed.
+
+End WithClasses.
+
+Hint Resolve range_set.
